---
title: Ex. 5.2
linktitle: Ex 5.2
type: book
date: "2021-01-02T00:00:00+01:00"
# Prev/next pager order (if `docs_section_pager` enabled in `params.toml`)
weight: 1
toc: false
---

???+ question "Ex. 5.2"
    Suppose that $B_{i,M}(x)$ is an order-$M$ $B$-spline defined in the Appendix on page 186 through the sequence (5.77)-(5.78).
    
    (a) Show by induction that $B_{i,M}(x) = 0$ for $x\not \in [\tau_i, \tau_{i+M}]$. This shows, for example, that the support of cubic $B$-splines is at most 5 knots.
    
    (b) Show by induction that $B_{i,M}(x) > 0$ for $x\in (\tau_i, \tau_{i+M})$. The $B$-splines are positive in the interior of their support.
    
    (c) Show by induction that $\sum_{i=1}^{K+M}B_{i,M}(x) = 1 \ \forall x\in [\xi_0, \xi_{K+1}]$.
    
    (d) Show that $B_{i,M}$ is a piecewise polynomial of order $M$ (degree M-1) on $[\xi_0, \xi_{K+1}]$, with breaks only at the knots $\xi_1,...,\xi_K$.
    
    (e) Show that an order-$M$ $B$-spline basis function is the density function of a convolution of $M$ uniform random variables.

???+ warning 
    In (e), the claim does not seem to be true unless $\tau_{i+1}-\tau_{i}=1$. See details below.

???+ done "Soln. 5.2"
    (a) For $B_{i,1}(x)$, by (5.77) we know that $B_{i,1}=0$ for $x\not \in [\tau_1, \tau_2]$. Assume that $B_{i, m-1}(x)=0$ for $x\not\in [\tau_i, \tau_{i+m-1}]$. If $x\not \in [\tau_i, \tau_{i+m}]$, then $x\not \in [\tau_i, \tau_{i+m-1}]$, thus $B_{i, m-1}(x) =0$ by our assumption. Similarly $x\not\in [\tau_{i+1}, \tau_{i+m}]$, thus $B_{i+1, m-1}(x) = 0$ by our assumption again. Therefore, by (5.78), for $x\not \in [\tau_i, \tau_{i+m}]$, we have $B_{i,m}(x) = 0$. By mathematical induction, the proof is complete. 

    For cubic $B$-splines, $M=4$, their support is at most $\tau_1, \tau_2, ..., \tau_5$, i.e., at most 5 knots.

    (b) For $B_{i,1}(x)$, by (5.77), $B_{i,1}(x) = 1 > 0$ for $x\in (\tau_1, \tau_2)$. Assume that $B_{i,m-1}(x) > 0$ for $x\in (\tau_{i}, \tau_{i+m-1})$. For any $x\in (\tau_i, \tau_{i+m})$, either $x\in (\tau_i, \tau_{i+m-1})$ or $x\in (\tau_{i+1}, \tau_{i+m})$. In either case, by (5.78) and our assumption, we have $B_{i, m}(x) > 0$. Therefore, the proof is complete.

    (c) Note, in this question we use superscript to differentiate $B$-spline base functions for different orders $M$ when necessary, b/c they can have different number of pre-&post-$\tau$. When $M=1$, by (5.77) we have $\sum_{i=1}^{K+1}B^{(1)}_{i,1}(x) = 1$ for $x\in [\xi_0,\xi_{K+1}]$. Suppose that the same holds for $M-1$, i.e., $\sum_{i=1}^{K+M-1}B^{(M-1)}_{i, M-1}(x)=1$ for $x\in [\xi_0, \xi_{K+1}]$.

    Let's move to the case $M$ now. 
    By (a), we have $B^{(M)}_{1, M-1}(x) =0$ for $x\not\in (\tau^{(M)}_1, \tau^{(M)}_{M})$, thus also for $x\in [\xi_0,\xi_{K+1}]$ ($\tau^{(M)}_M \le \xi_0$). Similarly, $B^{(M)}_{K+M+1, M-1}(x)=B^{(M-1)}_{K+M, M-1}(x)=0$ for $x\notin(\tau^{(M-1)}_{K+1+M-1}, \tau^{(M-1)}_{K+1+2*(M-1)})$, thus for $x\in [\xi_0,\xi_{K+1}]$ ($\xi_{K+1} \le \tau^{(M-1)}_{K+1+M-1}$).

    By (5.78), we have $x \in [\xi_0,\xi_{K+1}]$

    \begin{eqnarray}
    \sum_{i=1}^{K+M}B^{(M)}_{i,M}(x) &=& \sum_{i=1}^{K+M}\left[\frac{x-\tau_i}{\tau_{i+M-1}-\tau_i}B^{(M)}_{i,M-1}(x) + \frac{\tau_{i+M}-x}{\tau_{i+M}-\tau_{i+1}}B^{(M)}_{i+1, M-1}(x)\right]\non\\
    &=&\sum_{i=1}^{K+M}\frac{x-\tau_i}{\tau_{i+M-1}-\tau_i}B^{(M)}_{i, M-1}(x) + \sum_{i=1}^{K+M-1}\frac{\tau_{i+M}-x}{\tau_{i+M}-\tau_{i+1}}B^{(M)}_{i+1, M-1}(x)\non\\
    &=&\sum_{i=2}^{K+M}\frac{x-\tau_i}{\tau_{i+M-1}-\tau_i}B^{(M)}_{i, M-1}(x) + \sum_{i=2}^{K+M}\frac{\tau_{i+M-1}-x}{\tau_{i+M-1}-\tau_{i}}B^{(M)}_{i, M-1}(x)\non\\ 
		    &=&\sum_{i=2}^{K+M} \left(\frac{x-\tau_i}{\tau_{i+M-1}-\tau_i} + \frac{\tau_{i+M-1}-x}{\tau_{i+M-1}-\tau_{i}}\right)B^{(M)}_{i, M-1}(x)\non\\
		    &=&\sum_{i=2}^{K+M}B^{(M)}_{i, M-1}(x)\non\\
            &=&\sum_{i=2}^{K+M}B^{(M-1)}_{i-1, M-1}(x)\non\\
            &=&\sum_{i=1}^{K+M-1}B^{(M-1)}_{i, M-1}(x)\non\\
		    &=&1.\non
    \end{eqnarray}

    Thus the proof is complete.

    (d) Again we use induction. When $M=1$, by (5.77), $B_{i,1}$ is a piecewise polynomial of order 1 on $[\xi_0, \xi_{K+1}]$ with breaks only at the knots $\xi_1,...,\xi_K$. Suppose the same holds true for $M=m-1$, by (5.78), $B_{i,m}$ increases 1 order because $x$ multipliy by $B_{i,m-1}(x)$ in both summands. It's easy to see the break points remain the same.

    (e) Note that the claim does not seem to be true unless $\tau_{i+1}-\tau_{i}=1$. For example, consider $B_{i,1}(x) = \bb{1}([\tau_i, \tau_{i+1}))$. We have 
		
    \begin{equation}
        \int B_{i,1}(x)dx = \tau_{i+1} - \tau_i.\non
    \end{equation}

    So unless $\tau_{i+1}-\tau_i=1$, $B_{i,1}$ is not a density function. With this condition, we see that (5.78) in the text reduces to 

    \begin{equation}
			B_{i,m}(x) = \frac{x-\tau_i}{m-1}B_{i,m-1}(x) + \frac{\tau_{i+m}-x}{m-1}B_{i+1,m-1}(x),\non
    \end{equation}

    for each $i=1,...,K+2M-m$. 

    Now it's easy to verify that $B_{i,m}$ is a convolution of $B_{i,m-1}$ and the density function, denoted as $f$, of $U(0,1)$ where $U$ is uniformly distributed on $[0,1]$, thus the claim is true. For example, when $m=2$, by the definition above, we have

    \begin{equation}
        B_{i,2}(x) = \begin{cases}
            x - \tau_i & \text{ if } x\in [\tau_i, \tau_{i+1})\non\\
            \tau_{i+2} - x & \text{ if } x\in [\tau_{i+1}, \tau_{i+2})\non\\
            0 & \text{otherwise}.
        \end{cases}
    \end{equation} 

    On the other hand, it's easy to verify that

    \begin{equation}
        \int f(x-y)B_{i,1}(y)dy = \begin{cases}
            x - \tau_i & \text{ if } x\in [\tau_i, \tau_{i+1})\non\\
            \tau_{i+2} - x & \text{ if } x\in [\tau_{i+1}, \tau_{i+2})\non\\
            0 & \text{otherwise}.
        \end{cases}
    \end{equation}

    So we know that the claim holds for $m=2$.

    (e) Refer to [link](https://math.stackexchange.com/questions/3218351/b-splines-and-sum-of-uniform-variables).
    For convenience, we define that $\tau^{(M)}_1=\tau^{(M)}_2=\cdots=\tau^{(M)}_M=0$, $\tau^{(M)}_{M+k}=k$, $\forall k \in \{1,2,\cdots,K\}$, and $\tau^{(M)}_{M+K+1}=\tau^{(M)}_{M+K+2}=\cdots=\tau^{(M)}_{M+2K}=K+1$, $K\ge M$. (Here, we know that $B^{(M)}_{M+K+1, m}=0$, $\forall m \in \{1, 2, \cdots, min(K-1, M)\}$).

    Then, we know that $B^{(M)}_{M+k, 1}(x+k)$ is the density of $1$ random variable that follows $U(0, 1)$, $\forall k \in \{0,1,\cdots,K\}$.

    Suppose that $B^{(M)}_{M+k,m}(x+k)$ is the density function of a convolution of $m$ random variables $\sim U(0,1)$, $\forall 1\le m \le M$, $k \in \{0,1,\cdots, K-m+1\}$, we want to prove that $B^{(M+1)}_{M+1+k, M+1}(x+k)$ is the density function of a convolution of $M+1$ random variables $~U(0,1)$ by induction, $k\in \{0, 1, \cdots, K-M\}$.

    \begin{eqnarray}
        B^{(M+1)}_{M+1+k,M+1}(x+k) &=&
            \frac{x+k-\tau_{M+k}}{\tau_{2M+k}-\tau_{M+k}} B^{(M+1)}_{M+k,M}(x+k) + \frac{\tau_{2M+k+1}-x-k}{\tau_{2M+k+1}-\tau_{M+k+1}}B^{(M+1)}_{M+k+2,M}(x+k)\non\\
            &=&\frac{x}{M}B^{(M+1)}_{M+k+1,M}(x+k)+\frac{M+1-x}{M}B^{(M+1)}_{M+k+2,M}(x+k)\non\\
            &=&\frac{x}{M}B^{(M+1)}_{M+1,M}(x)+\frac{M+1-x}{M}B^{(M+1)}_{M+2,M}(x)\non\\
            &=&\frac{x}{M}B^{(M)}_{M,M}(x)+\frac{M+1-x}{M}B^{(M)}_{M,M}(x-1)\non\\
            &=&B^{(M+1)}_{M+1, M+1}(x)\non
    \end{eqnarray}

    Thus, we only need to prove that $B^{(M+1)}_{M+1, M+1}(x)$ is the density function of a convolution of $M+1$ random variables $\sim U(0, 1)$.
    
    Using the characteristic function, we can write $\forall u \in [0, M]$

    \begin{eqnarray}
        f_{X_1+\cdots+X_M}(u) = \mathcal{F}^{-1}\left[\left(\frac{i(1-\exp{it})}{t}\right)^M\right](u)\non
    \end{eqnarray}

    After calculation, we have $\forall u \in [0, M]$

    \begin{eqnarray}
        f_{X_1+\cdots+X_M}(u) = \frac{1}{2(M-1)!}\sum_{k=0}^{M}(-1)^k\binom{M}{k}(u-k)^{M-1}sgn(u-k)\non
    \end{eqnarray}

    If we have $B^{(M)}_{M,M}(x) = \frac{1}{2(M-1)!}\sum_{k=0}^{M}(-1)^k\binom{M}{k}(x-k)^{M-1}sgn(x-k)$, then

    \begin{eqnarray}
    &&\frac{x}{M}B^{(M)}_{M,M}(x)+\frac{M+1-x}{M}B^{(M)}_{M,M}(x-1)\non\\
        &=&\frac{x}{M}f_{X_1+\cdots+X_M}(x)+\frac{M+1-x}{M}f_{X_1+\cdots+X_M}(x-1)\non\\
        &=&\frac{x}{M}\frac{1}{2(M-1)!}\sum_{k=0}^{M}(-1)^k\binom{M}{k}(x-k)^{M-1}sgn(x-k)\non\\ 
        &+& \frac{M+1-x}{M} \frac{1}{2(M-1)!}\sum_{k=0}^{M}(-1)^k\binom{M}{k}(x-1-k)^{M-1}sgn(x-1-k)\non\\
        &=&\frac{x}{2M!}\sum_{k=0}^{M}(-1)^k\binom{M}{k}(x-k)^{M-1}sgn(x-k)\non\\ 
        &-&\frac{M+1-x}{2M!}\sum_{k=1}^{M+1}(-1)^k\binom{M}{k-1}(x-k)^{M-1}sgn(x-k)\non\\
        &=&\frac{x}{2M!}\sum_{k=0}^{M+1}(-1)^k\left[\binom{M}{k}+\binom{M}{k-1}\right](x-k)^{M-1}sgn(x-k)\non\\
        &-&\frac{M+1}{2M!}\sum_{k=1}^{M+1}(-1)^k\binom{M}{k-1}(x-k)^{M-1}sgn(x-k)\non\\
        &=&\frac{x}{2M!}\sum_{k=0}^{M+1}(-1)^k\binom{M+1}{k}(x-k)^{M-1}sgn(x-k)\non\\
        &-&\frac{1}{2M!}\sum_{k=1}^{M+1}(-1)^kk\binom{M+1}{k}(x-k)^{M-1}sgn(x-k)\non\\
        &=&\frac{1}{2M!}\sum_{k=0}^{M+1}(-1)^k\binom{M+1}{k}(x-k)^{M}sgn(x-k)\non\\
        &=&f_{X_1+\cdots+X_{M+1}}(x)\non
    \end{eqnarray}

    So we have

    \begin{eqnarray}
        &&B^{(M+1)}_{M+1+k,M+1}(x+k)=B^{(M+1)}_{M+1, M+1}(x)\non\\
        &=&\frac{1}{2M!}\sum_{k=0}^{M+1}(-1)^k\binom{M+1}{k}(x-k)^{M}sgn(x-k)\non\\
        &=&f_{X_1+\cdots+X_{M+1}}(x), \forall k\in \{0, 1, \cdots, K-M\}\non
    \end{eqnarray}

    which is a density function of convolution of $M+1$ random variables $~U(0,1)$.

    Note that from this [post](https://math.stackexchange.com/questions/2680616/convolution-of-i-i-d-with-uniform-distribution), we know that 

    \begin{eqnarray}
        F_{X_1+\cdots+X_M}(u) = \frac{1}{M!}\sum_{k=0}^{M-1}(-1)^k\binom{M}{k}(u-k)^{M}_{+}\non
    \end{eqnarray}

    So we can get

    \begin{eqnarray}
        f_{X_1+\cdots+X_M}(u) = F'_{X_1+\cdots+X_M}(u) = \frac{1}{(M-1)!}\sum_{k=0}^{M-1}(-1)^k\binom{M}{k}(u-k)^{M-1}sgn((u-k)_{+})\non
    \end{eqnarray}

    To prove that

    \begin{eqnarray}
        &&\frac{1}{(M-1)!}\sum_{k=0}^{M-1}(-1)^k\binom{M}{k}(u-k)^{M-1}sgn((u-k)_{+})\non\\
        &=&\frac{1}{2(M-1)!}\sum_{k=0}^{M}(-1)^k\binom{M}{k}(u-k)^{M-1}sgn(u-k)
    \end{eqnarray}
    
    We can use induction.

    For $M=2$, we have

    \begin{eqnarray}
        &&\frac{1}{(M-1)!}\sum_{k=0}^{M-1}(-1)^k\binom{M}{k}(x-k)^{M-1}sgn((x-k)_{+})\non\\
        &=& x \non\\
        &=&\frac{1}{2(M-1)!}\sum_{k=0}^{M}(-1)^k\binom{M}{k}(x-k)^{M-1}sgn(x-k), x\in (0,1)\non\\
        &&\frac{1}{(M-1)!}\sum_{k=0}^{M-1}(-1)^k\binom{M}{k}(x-k)^{M-1}sgn((x-k)_{+})\non\\
        &=& 2-x \non\\
        &=&\frac{1}{2(M-1)!}\sum_{k=0}^{M}(-1)^k\binom{M}{k}(x-k)^{M-1}sgn(x-k), x\in (1,2)\non\\
    \end{eqnarray}

    Assume that for $M$, the statement holds for $x\in (0, M)$. For $M+1$ and $x\in (0, M+1)$

    \begin{eqnarray}
        &&\frac{1}{M!}\sum_{k=0}^{M}(-1)^k\binom{M+1}{k}(x-k)^{M}sgn((x-k)_{+})\non\\
        &=&\frac{1}{M!}\sum_{k=0}^{M}(-1)^k\binom{M}{k}(x-k)^{M}sgn((x-k)_{+})+\frac{1}{M!}\sum_{k=1}^{M}(-1)^k\binom{M}{k-1}(x-k)^{M}sgn((x-k)_{+})\non\\
        &=&\frac{1}{M!}\sum_{k=0}^{M-1}(-1)^k\binom{M}{k}(x-k)^{M}sgn((x-k)_{+})+\frac{1}{M!}\sum_{k=1}^{M}(-1)^k\binom{M}{k-1}(x-k)^{M}sgn((x-k)_{+})\non\\
        &=&\frac{x}{2M!}\sum_{k=0}^{M}(-1)^k\binom{M}{k}(x-k)^{M-1}sgn(x-k)-\frac{1}{(M-1)!}\sum_{k=1}^{M}(-1)^k\binom{M-1}{k-1}(x-k)^{M-1}sgn((x-k)_{+})\non\\
        &+&\frac{x-1}{2M!}\sum_{k=1}^{M+1}(-1)^k\binom{M}{k-1}(x-k)^{M-1}sgn(x-k)-\frac{1}{(M-1)!}\sum_{k=2}^{M+1}(-1)^k\binom{M-1}{k-2}(x-k)^{M-1}sgn((x-k)_{+})\non\\
        &=&\frac{x}{2M!}\sum_{k=0}^{M+1}(-1)^k\binom{M+1}{k}(x-k)^{M-1}sgn(x-k)-\frac{1}{2M!}\sum_{k=1}^{M+1}(-1)^k\binom{M}{k-1}(x-k)^{M-1}sgn(x-k)\non\\
        &-&\frac{1}{(M-1)!}\sum_{k=1}^{M+1}(-1)^k\binom{M}{k-1}(x-k)^{M-1}sgn((x-k)_{+})\non\\
        &=&\frac{x}{2M!}\sum_{k=0}^{M+1}(-1)^k\binom{M+1}{k}(x-k)^{M-1}sgn(x-k)-\frac{1}{2M!}\sum_{k=1}^{M+1}(-1)^k\binom{M}{k-1}(x-k)^{M-1}sgn(x-k)\non\\
        &-&\frac{1}{2(M-1)!}\sum_{k=1}^{M+1}(-1)^k\binom{M}{k-1}(x-k)^{M-1}sgn(x-k)\non\\
        &=&\frac{x}{2M!}\sum_{k=0}^{M+1}(-1)^k\binom{M+1}{k}(x-k)^{M-1}sgn(x-k)-\frac{1}{2M!}\sum_{k=1}^{M+1}(-1)^k\binom{M+1}{k}k(x-k)^{M-1}sgn(x-k)\non\\
        &=&\frac{1}{2M!}\sum_{k=0}^{M+1}(-1)^k\binom{M+1}{k}(x-k)^{M}sgn(x-k)\non
    \end{eqnarray}

    which completes the proof.

    Actually, the above proof is not rigorous, b/c it only holds for $x\in (1,M)$. We need to consider $x\in (0,1)$ and $x\in (M,M+1)$. For $x\in (0,1)$, we need to prove the following identity ($\forall x\in \mathbb{R}$):

    \begin{eqnarray}
        \sum_{k=1}^M(-1)^k\binom{M}{k}(x-k)^{M-1} = -x^{(M-1)}\non
    \end{eqnarray}

    This can be proved by induction too, and actually it depends on another identity ($\forall x\in \mathbb{R}$):

    \begin{eqnarray}
        \sum_{k=0}^M(-1)^k\binom{M}{k}(x-k)^{M-1} = 0\non
    \end{eqnarray}
    
    A scatch of the proof is following:

    \begin{eqnarray}
        &&\sum_{k=0}^{M+1}(-1)^k\binom{M+1}{k}(x-k)^{M}\non\\
        &=&\sum_{k=0}^{M}(-1)^k\binom{M}{k}(x-k)^{M}+\sum_{k=1}^{M+1}(-1)^k\binom{M}{k-1}(x-k)^{M}\non\\
        &=&-M\sum_{k=1}^{M}(-1)^k\binom{M-1}{k-1}(x-k)^{M-1}+\sum_{k=1}^{M+1}(-1)^k\binom{M}{k-1}(x-k)^{M}\non\\
        &=&-M\sum_{k=1}^{M}(-1)^k\binom{M-1}{k-1}(x-k)^{M-1}-M\sum_{k=2}^{M+1}(-1)^k\binom{M-1}{k-2}(x-k)^{M-1}\non\\
        &+&(x-1)\sum_{k=1}^{M+1}(-1)^k\binom{M}{k-1}(x-k)^{M-1}\non\\
        &=&-M\sum_{k=1}^{M}(-1)^k\binom{M-1}{k-1}(x-k)^{M-1}-M\sum_{k=2}^{M+1}(-1)^k\binom{M-1}{k-2}(x-k)^{M-1}\non\\
        &-&(x-1)\sum_{k=0}^{M}(-1)^k\binom{M}{k}(x-k-1)^{M-1}\non\\
        &=&M\sum_{k=0}^{M-1}(-1)^k\binom{M-1}{k}(x-k-1)^{M-1}+M\sum_{k=1}^{M}(-1)^k\binom{M-1}{k-1}(x-k-1)^{M-1}\non\\
        &=&M\sum_{k=0}^{M}(-1)^k\binom{M}{k}(x-k-1)^{M-1}\non\\
        &=&0\non
    \end{eqnarray}
    
    Those two identities may be able to simplify the derivation above. Actually, to prove equation $(1)$, we notice that 

    \begin{eqnarray}
        &&\frac{1}{2(M-1)!}\sum_{k=0}^{M}(-1)^k\binom{M}{k}(u-k)^{M-1}sgn(u-k) \non\\
        &=&\frac{1}{2(M-1)!}\sum_{k=0}^{M}(-1)^k\binom{M}{k}(u-k)^{M-1}(sgn((u-k)_{+})-sgn((u-k)_{-}))\non
    \end{eqnarray}

    And

    \begin{eqnarray}
        &&\frac{1}{2(M-1)!}\sum_{k=0}^{M}(-1)^k\binom{M}{k}(u-k)^{M-1}(sgn((u-k)_{+})+sgn((u-k)_{-}))\non\\ 
        &=& \frac{1}{2(M-1)!}\sum_{k=0}^{M}(-1)^k\binom{M}{k}(u-k)^{M-1}=0\non
    \end{eqnarray}

    So, we easily got the result of equation $(1)$.
